Finalising SN proof and working on constructions

src/PlutusIR/Semantics/Static/normaliser_STLC/alpha/alpha_typing.v
@@ -1,14 +1,16 @@
 Require Import Coq.Lists.List.
 Require Import Coq.Strings.String.
 Import ListNotations.
-From PlutusCert Require Import freshness util alpha STLC_named STLC_named_typing Util.List alpha_freshness alpha_rename.
+From PlutusCert Require Import freshness util alpha.alpha STLC_named STLC_named_typing Util.List alpha_freshness alpha_rename.
 Local Open Scope string_scope.
 Local Open Scope list_scope.
+
+From PlutusCert Require PlutusIR.
 
 (* Alpha equivalence of types *)
 
 (* Contextual alpha equivalence: kinding contexts that match alpha contexts*)
-Inductive CAlpha : list (string * string) -> list (string * type) -> list (string * type) -> Prop :=
+Inductive CAlpha : list (string * string) -> list (string * PlutusIR.kind) -> list (string * PlutusIR.kind) -> Prop :=
   | calpha_nil D : CAlpha [] D D (* Non-empty kinding enviornments because id renamings are like no renamings. TODO: think whether we want to allow that or want to enforce that id renamings are in the alpha enviornment always*)
   | calpha_cons x y K sigma Gamma Gamma' :
     CAlpha sigma Gamma Gamma' ->
@@ -17,9 +19,11 @@ Inductive CAlpha : list (string * string) -> list (string * type) -> list (strin
     CAlpha sigma Gamma Gamma' ->
     CAlpha sigma ((x, K)::Gamma) ((x, K)::Gamma'). *)
 
+Set Printing Implicit.
+
 (* Exercise and possibly useful *)
 Lemma alpha_preserves_typing sigma s t A Gamma Gamma' :
-  Alpha sigma s t -> CAlpha sigma Gamma Gamma' -> Gamma |-* s : A -> Gamma' |-* t : A.
+  Alpha sigma s t -> CAlpha sigma Gamma Gamma' -> STLC_named_typing.has_kind Gamma s A -> STLC_named_typing.has_kind Gamma' t A.
 Proof.
   intros HAlpha Htype.
   generalize dependent A.
@@ -62,17 +66,51 @@ Proof.
            specialize (IHa H Hlookup).
            assumption.
   - intros Gamma' Gamma HCAlpha A0 HType.
-    inversion HType.
+    inversion HType; subst;
     specialize (IHHAlpha ((y, A)::Gamma') ((x, A)::Gamma)
-      (calpha_cons x y A sigma Gamma Gamma' HCAlpha) K2 H4).
-    apply K_Lam.
-    assumption.
+      (calpha_cons x y A sigma Gamma Gamma' HCAlpha) _ H5); constructor; auto.
   - intros Gamma' Gamma HCAlpha A HType. 
-    inversion HType.
-    specialize (IHHAlpha1 Gamma' Gamma HCAlpha (tp_arrow K1 A) H2).
-    specialize (IHHAlpha2 Gamma' Gamma HCAlpha K1 H4).
-    apply K_App with (K1 := K1); assumption.
+    inversion HType; subst; econstructor; eauto.
+  - intros.
+    inversion H; subst.
+    constructor. auto.
 Qed.
+
+
+
+
+
+
+
+
+
+
+
+
+
+
+
+
+
+
+
+
+
+
+
+
+
+(* TODO, Kind of old code below*)
+
+
+
+
+
+
+
+
+
+
 
 (* FROM deadcode/DSP/lemmas.v*)
   Lemma strengthen_Γ_cons Γ t T x Tx :
@@ -89,7 +127,7 @@ Theorem substituteTCA_preserves_kinding : forall T Delta X K U L,
     Delta |-* U : L ->
     Delta |-* (substituteTCA X U T) : K.
 Proof with eauto.
-  induction T.
+  (* induction T.
   all: intros Delta X K U L Hkind__T HHkind__U.
   all: autorewrite with substituteTCA.
   all: simpl.
@@ -143,7 +181,7 @@ Proof with eauto.
         -- (* Y not in U, so we can remove (Y, t) from the context *)
           admit.
   - (* Ty_App *)
-    admit.
+    admit. *)
 Admitted.
 
 (* TODO: See also Theorems/Weakening for already existing PIR version
@@ -187,6 +225,7 @@ Proof.
       now apply not_ftv_app_not_left in H0.
     + eapply IHT'2; eauto.
       now apply not_ftv_app_not_right in H0.
+  - auto.
 Qed.
 
 Corollary substituteTCA_vacuous_specialized X U T:  
@@ -213,7 +252,7 @@ Theorem substituteTCA_preserves_kinding_alpha_ren : forall T Delta Delta' ren T'
     Delta' |-* U' : L ->
     Delta' |-* (substituteTCA X' U' T') : K.
 Proof with eauto.
-  induction T.
+  (* induction T.
   all: intros Delta Delta' ren T' X X' K U' L HalphaT HalphaX HalphaC Hkind__T HHkind__U.
   all: autorewrite with substituteTCA.
   all: simpl.
@@ -316,8 +355,8 @@ Proof with eauto.
     autorewrite with substituteTCA.
     eapply K_App.
     + eapply IHT1; eauto.
-    + eapply IHT2; eauto.
-Qed.
+    + eapply IHT2; eauto. *)
+Admitted.
 
 Corollary substituteTCA_preserves_kinding_specialised : forall T Delta X K U L,
     ((X, L) :: Delta) |-* T : K ->
